src/arch/x64/X64.Semantics_s.fst
@@ -30,6 +30,7 @@ type ocmp =
 type code = precode ins ocmp
 type codes = list code
 
+[@va_qattr]
 noeq type state = {
   ok: bool;
   regs: reg -> nat64;
@@ -45,6 +46,7 @@ assume val havoc : state -> ins -> nat64
 unfold let eval_reg (r:reg) (s:state) : nat64 = s.regs r
 unfold let eval_mem (ptr:int) (s:state) : nat64 = load_mem64 ptr s.mem
 
+[@va_qattr]
 let eval_maddr (m:maddr) (s:state) : int =
   let open FStar.Mul in
     match m with
